Added location for ssprove and mutable bool for idents

language/src/ast_to_rustspec.rs
@@ -409,7 +409,8 @@ fn translate_expr_expects_exp(
     specials: &SpecialNames,
     e: &Expr,
 ) -> TranslationResult<Spanned<Expression>> {
-    match translate_expr(sess, specials, e)? {
+    let expr = translate_expr(sess, specials, e)?;
+    Ok(match expr {
         (ExprTranslationResult::TransExpr(e), span) => Ok((e, span)),
         (ExprTranslationResult::TransStmt(_), span) => {
             sess.span_rustspec_err(
@@ -418,7 +419,7 @@ fn translate_expr_expects_exp(
             );
             Err(())
         }
-    }
+    }?)
 }
 
 fn translate_function_argument(
@@ -433,12 +434,18 @@ fn translate_function_argument(
                 Err(())
             }
             Mutability::Not => Ok((
-                translate_expr_expects_exp(sess, specials, e1)?,
+                {
+                    let trans = translate_expr_expects_exp(sess, specials, e1)?;
+                    trans
+                },
                 (Borrowing::Borrowed, e.span.clone().into()),
             )),
         },
         _ => Ok((
-            translate_expr_expects_exp(sess, specials, e)?,
+            {
+                let trans = translate_expr_expects_exp(sess, specials, e)?;
+                trans
+            },
             (Borrowing::Consumed, e.span.clone().into()),
         )),
     }
@@ -548,30 +555,39 @@ fn translate_expr(
     e: &Expr,
 ) -> TranslationResult<Spanned<ExprTranslationResult>> {
     match &e.kind {
-        ExprKind::Binary(op, e1, e2) => Ok((
-            ExprTranslationResult::TransExpr(Expression::Binary(
-                (translate_binop(op.clone().node), op.clone().span.into()),
-                Box::new(translate_expr_expects_exp(sess, specials, e1)?),
-                Box::new(translate_expr_expects_exp(sess, specials, e2)?),
-                None,
-            )),
-            e.span.into(),
-        )),
-        ExprKind::Unary(op, e1) => Ok((
-            ExprTranslationResult::TransExpr(Expression::Unary(
-                match *op {
-                    UnOp::Not => UnOpKind::Not,
-                    UnOp::Neg => UnOpKind::Neg,
-                    UnOp::Deref => {
-                        sess.span_rustspec_err(e.span, "dereferences not allowed in Hacspec");
-                        return Err(());
-                    }
-                },
-                Box::new(translate_expr_expects_exp(sess, specials, e1)?),
-                None,
-            )),
-            e.span.into(),
-        )),
+        ExprKind::Binary(op, e1, e2) => {
+            let trans_e1 = translate_expr_expects_exp(sess, specials, e1)?;
+            let trans_e2 = translate_expr_expects_exp(sess, specials, e2)?;
+
+            Ok((
+                ExprTranslationResult::TransExpr(Expression::Binary(
+                    (translate_binop(op.clone().node), op.clone().span.into()),
+                    Box::new(trans_e1),
+                    Box::new(trans_e2),
+                    None,
+                )),
+                e.span.into(),
+            ))
+        }
+        ExprKind::Unary(op, e1) => {
+            let trans = translate_expr_expects_exp(sess, specials, e1)?;
+
+            Ok((
+                ExprTranslationResult::TransExpr(Expression::Unary(
+                    match *op {
+                        UnOp::Not => UnOpKind::Not,
+                        UnOp::Neg => UnOpKind::Neg,
+                        UnOp::Deref => {
+                            sess.span_rustspec_err(e.span, "dereferences not allowed in Hacspec");
+                            return Err(());
+                        }
+                    },
+                    Box::new(trans),
+                    None,
+                )),
+                e.span.into(),
+            ))
+        }
         ExprKind::Path(Some(_), _) => {
             sess.span_rustspec_err(e.span, "trait associated values not allowed in Hacspec");
             Err(())
@@ -610,7 +626,7 @@ fn translate_expr(
                 e.span.into(),
             ))
         }
-        ExprKind::Path(None, path) => translate_expr_name(sess, path, &e.span, specials),
+        ExprKind::Path(None, path) => Ok(translate_expr_name(sess, path, &e.span, specials)?),
         ExprKind::Call(func, args) => {
             let func_name_kind = match &func.kind {
                 ExprKind::Path(None, path) => Ok(translate_func_name(sess, specials, &path)?),
@@ -692,6 +708,7 @@ fn translate_expr(
                                     .map(|cell| translate_expr_expects_exp(sess, specials, &cell))
                                     .collect();
                                 let new_cells = check_vec(new_cells)?;
+
                                 return Ok((
                                     (ExprTranslationResult::TransExpr(Expression::NewArray(
                                         Some(func_name_but_as_type),
@@ -746,6 +763,7 @@ fn translate_expr(
                                                                 (Borrowing::Consumed, i.1.clone()),
                                                             )],
                                                             None,
+                                                            vec![],
                                                         ),
                                                         i.1.clone(),
                                                     )
@@ -787,6 +805,7 @@ fn translate_expr(
                                                                 (Borrowing::Consumed, i.1.clone()),
                                                             )],
                                                             None,
+                                                            vec![],
                                                         ),
                                                         i.1.clone(),
                                                     )
@@ -842,6 +861,7 @@ fn translate_expr(
                             func_name,
                             func_args,
                             None,
+                            vec![],
                         )),
                         e.span.into(),
                     ))
@@ -899,11 +919,12 @@ fn translate_expr(
                     method_name,
                     rest_args_final,
                     None,
+                    vec![],
                 )),
                 e.span.into(),
             ))
         }
-        ExprKind::Lit(lit) => translate_literal(sess, lit, e.span.clone()),
+        ExprKind::Lit(lit) => Ok(translate_literal(sess, lit, e.span.clone())?),
         ExprKind::Assign(lhs, rhs_e, _) => {
             let (r_e, r_e_question_mark) =
                 match translate_expr_accepts_question_mark(sess, specials, &rhs_e)? {
@@ -957,6 +978,7 @@ fn translate_expr(
                         }
                         (ExprTranslationResult::TransExpr(r_index), span) => Ok((r_index, span)),
                     };
+
                     match &a.kind {
                         ExprKind::Path(None, path) => match path.segments.as_slice() {
                             [var] => match &var.args {
@@ -1015,13 +1037,13 @@ fn translate_expr(
                 }
                 (ExprTranslationResult::TransExpr(r_cond), span) => Ok((r_cond, span)),
             }?;
-            let mut r_t_e = translate_block(sess, specials, t_e)?;
-            let r_f_e = match f_e {
+            let mut block_r_t_e = translate_block(sess, specials, t_e)?;
+            let block_r_f_e = match f_e {
                 None => Ok(None),
                 Some(f_e) => match &f_e.kind {
                     ExprKind::Block(f_e, _) => {
-                        let r_f_e = translate_block(sess, specials, f_e)?;
-                        Ok(Some(r_f_e))
+                        let block_r_f_e = translate_block(sess, specials, f_e)?;
+                        Ok(Some(block_r_f_e))
                     }
                     _ => {
                         sess.span_rustspec_err(
@@ -1035,21 +1057,22 @@ fn translate_expr(
             let stmt_result = (
                 ExprTranslationResult::TransStmt(Statement::Conditional(
                     r_cond.clone(),
-                    r_t_e.clone(),
-                    r_f_e.clone(),
+                    block_r_t_e.clone(),
+                    block_r_f_e.clone(),
                     None,
                 )),
                 e.span.into(),
             );
+
             // Now, we determine whether what we have translate is an inline conditional
             // or a statement-like conditional
-            match r_f_e {
-                Some(mut r_f_e) => {
-                    if r_t_e.0.stmts.len() == 1 && r_f_e.0.stmts.len() == 1 {
-                        let r_t_span = r_t_e.1.clone();
-                        let r_f_span = r_f_e.1.clone();
-                        let r_t_e = r_t_e.0.stmts.pop().unwrap();
-                        let r_f_e = r_f_e.0.stmts.pop().unwrap();
+            match block_r_f_e {
+                Some(mut block_r_f_e) => {
+                    if block_r_t_e.0.stmts.len() == 1 && block_r_f_e.0.stmts.len() == 1 {
+                        let r_t_span = block_r_t_e.1.clone();
+                        let r_f_span = block_r_f_e.1.clone();
+                        let r_t_e = block_r_t_e.0.stmts.pop().unwrap();
+                        let r_f_e = block_r_f_e.0.stmts.pop().unwrap();
                         match (r_t_e, r_f_e) {
                             (
                                 (Statement::ReturnExp(r_t_e), _),
@@ -1085,10 +1108,11 @@ fn translate_expr(
                     Err(())
                 }
             };
-            let e_begin_end = match &range.kind {
+            let (e_begin, e_end) = match &range.kind {
                 ExprKind::Range(Some(r_begin), Some(r_end), RangeLimits::HalfOpen) => {
                     let e_begin = translate_expr(sess, specials, r_begin)?;
                     let e_end = translate_expr(sess, specials, r_end)?;
+
                     match (e_begin, e_end) {
                         (
                             (ExprTranslationResult::TransExpr(e_begin), span_begin),
@@ -1110,11 +1134,13 @@ fn translate_expr(
                     );
                     Err(())
                 }
-            };
-            let (e_begin, e_end) = e_begin_end?;
-            let r_b = translate_block(sess, specials, b)?;
+            }?;
+            let block_r_b = translate_block(sess, specials, b)?;
+
             Ok((
-                ExprTranslationResult::TransStmt(Statement::ForLoop(id?, e_begin, e_end, r_b)),
+                ExprTranslationResult::TransStmt(Statement::ForLoop(
+                    id?, e_begin, e_end, block_r_b,
+                )),
                 e.span.into(),
             ))
         }
@@ -1160,14 +1186,17 @@ fn translate_expr(
         ExprKind::Tup(args) => {
             let r_args = args
                 .into_iter()
-                .map(|arg| match translate_expr(sess, specials, arg)? {
-                    (ExprTranslationResult::TransExpr(r_arg), r_span) => Ok((r_arg, r_span)),
-                    (ExprTranslationResult::TransStmt(_), r_span) => {
-                        sess.span_rustspec_err(
-                            r_span,
-                            "statements forbidden in tuple expressions in Hacspec",
-                        );
-                        Err(())
+                .map(|arg| {
+                    let expr = translate_expr(sess, specials, arg)?;
+                    match expr {
+                        (ExprTranslationResult::TransExpr(r_arg), r_span) => Ok((r_arg, r_span)),
+                        (ExprTranslationResult::TransStmt(_), r_span) => {
+                            sess.span_rustspec_err(
+                                r_span,
+                                "statements forbidden in tuple expressions in Hacspec",
+                            );
+                            Err(())
+                        }
                     }
                 })
                 .collect();
@@ -1328,6 +1357,7 @@ fn translate_expr(
                     })
                     .collect(),
             )?;
+
             Ok((
                 ExprTranslationResult::TransExpr(Expression::MatchWith(Box::new(e1), arms)),
                 e.span.clone().into(),
@@ -1412,6 +1442,7 @@ fn translate_expr(
             };
             let new_e1 = translate_expr_expects_exp(sess, specials, e1)?;
             let new_e2 = translate_expr_expects_exp(sess, specials, e2)?;
+
             Ok((
                 ExprTranslationResult::TransExpr(Expression::Tuple(vec![new_e1, new_e2])),
                 e.span.into(),
@@ -1481,6 +1512,7 @@ fn translate_expr(
                                                     (Borrowing::Consumed, i.1.clone()),
                                                 )],
                                                 Some(vec![BaseTyp::UInt8]),
+                                                vec![],
                                             ),
                                             i.1.clone(),
                                         )
@@ -1614,9 +1646,10 @@ fn translate_expr_accepts_question_mark(
 
 fn translate_pattern(sess: &Session, pat: &Pat) -> TranslationResult<Spanned<Pattern>> {
     match &pat.kind {
-        PatKind::Ident(BindingMode::ByValue(_), id, None) => {
-            Ok((Pattern::IdentPat(translate_ident(id).0), pat.span.into()))
-        }
+        PatKind::Ident(BindingMode::ByValue(m), id, None) => Ok((
+            Pattern::IdentPat(translate_ident(id).0, m.clone() == Mutability::Mut),
+            pat.span.into(),
+        )),
         PatKind::TupleStruct(None, path, args) => {
             let struct_name = translate_struct_name(sess, path)?;
             if args.len() == 1 {
@@ -1693,7 +1726,9 @@ fn translate_statement(
                     Err(())
                 }
                 LocalKind::Init(e) => {
-                    match translate_expr_accepts_question_mark(sess, specials, &e)? {
+                    let expr = translate_expr_accepts_question_mark(sess, specials, &e)?;
+
+                    match expr {
                         (ExprTranslationResultMaybeQuestionMark::TransStmt(_), _) => {
                             sess.span_rustspec_err(
                                 e.span,
@@ -1708,20 +1743,23 @@ fn translate_statement(
                     }
                 }
             }?;
+
             Ok(vec![(
                 Statement::LetBinding(pat, ty, init, question_mark),
                 s.span.into(),
             )])
         }
         StmtKind::Expr(e) => {
-            let t_s = match translate_expr(sess, specials, &e)? {
+            let t_s = translate_expr(sess, specials, &e)?;
+            let t_s = match t_s {
                 (ExprTranslationResult::TransExpr(e), _) => Statement::ReturnExp(e),
                 (ExprTranslationResult::TransStmt(s), _) => s,
             };
             Ok(vec![(t_s, s.span.into())])
         }
         StmtKind::Semi(e) => {
-            let t_s = match translate_expr_accepts_question_mark(sess, specials, &e)? {
+            let t_s = translate_expr_accepts_question_mark(sess, specials, &e)?;
+            let t_s = match t_s {
                 (ExprTranslationResultMaybeQuestionMark::TransExpr(e, question_mark), span) => {
                     Statement::LetBinding((Pattern::WildCard, span), None, (e, span), question_mark)
                 }
@@ -1749,7 +1787,9 @@ fn translate_block(
         .iter()
         .map(|s| translate_statement(sess, specials, &s))
         .collect();
-    let stmts = check_vec(stmts)?.into_iter().flatten().collect();
+    let stmts = check_vec(stmts)?;
+    let stmts: Vec<_> = stmts.into_iter().flatten().collect();
+
     Ok((
         Block {
             stmts,
@@ -1758,6 +1798,8 @@ fn translate_block(
             contains_question_mark: None,
             // We initialize these fields to None as they are
             // to be filled by the typechecker
+            mutable_vars: vec![],
+            function_dependencies: vec![],
         },
         b.span.into(),
     ))
@@ -2522,6 +2564,8 @@ fn translate_items<F: Fn(&Vec<Spanned<String>>) -> ExternalData>(
                         return_typ: None,
                         mutated: None,
                         contains_question_mark: None,
+                        mutable_vars: Vec::new(),
+                        function_dependencies: Vec::new(),
                     },
                     i.span.into(),
                 ),
@@ -2531,6 +2575,8 @@ fn translate_items<F: Fn(&Vec<Spanned<String>>) -> ExternalData>(
             let fn_sig = FuncSig {
                 args: fn_inputs,
                 ret: fn_output,
+                mutable_vars: Vec::new(),
+                function_dependencies: Vec::new(),
             };
             let fn_item = Item::FnDecl(
                 translate_toplevel_ident(&i.ident, TopLevelIdentKind::Function),
