coq/src/Hacspec_Poly1305.v
@@ -1,4 +1,8 @@
 (** This file was automatically generated using Hacspec **)
+From Crypt Require Import choice_type Package Prelude.
+Import PackageNotation.
+From extructures Require Import ord fset.
+
 Require Import Hacspec_Lib MachineIntegers.
 From Coq Require Import ZArith.
 Import List.ListNotations.
@@ -10,7 +14,7 @@ Require Import Hacspec_Lib.
 Definition poly_key_t := nseq (uint8) (usize 32).
 
 Definition blocksize_v : uint_size :=
-  usize 16.
+  (usize 16).
 
 Definition poly_block_t := nseq (uint8) (usize 16).
 
@@ -23,121 +27,283 @@ Notation "'block_index_t'" := (uint_size) : hacspec_scope.
 Definition field_canvas_t := nseq (int8) (17).
 Definition field_element_t := nat_mod 0x03fffffffffffffffffffffffffffffffb.
 
-Notation "'poly_state_t'" := ((field_element_t × field_element_t × poly_key_t
+Notation "'poly_state_t'" := ((
+  field_element_t '×
+  field_element_t '×
+  poly_key_t
 )) : hacspec_scope.
 
-Definition poly1305_encode_r (b_435 : poly_block_t) : field_element_t :=
-  let n_436 : uint128 :=
-    uint128_from_le_bytes (array_from_seq (16) (array_to_seq (b_435))) in 
-  let n_436 :=
-    (n_436) .& (secret (
-        @repr WORDSIZE128 21267647620597763993911028882763415551) : int128) in 
-  nat_mod_from_secret_literal (n_436).
+Definition n_5_loc : Location :=
+  (choice_type_from_type uint128 ; 12%nat).
+Program Definition poly1305_encode_r
+  (b_0 : poly_block_t)
+  : code (fset [ n_5_loc]) [interface] (choice_type_from_type (
+      field_element_t)) :=
+  ({code
+     temp_2 ←
+      (array_from_seq (16) (array_to_seq (b_0))) ;; 
+    let temp_1 := type_from_choice_type_elem temp_2 in
+     temp_4 ←
+      (uint128_from_le_bytes (temp_1)) ;; 
+    let temp_3 := type_from_choice_type_elem temp_4 in
+    #put n_5_loc := choice_type_from_type_elem
+      (temp_3) ;;
+    n_5 ← get n_5_loc ;;
+    let n_5 := type_from_choice_type_elem (n_5) in
+     temp_7 ←
+      (secret (@repr WORDSIZE128 21267647620597763993911028882763415551)) ;; 
+    let temp_6 := type_from_choice_type_elem temp_7 : int128 in
+    let n_5 :=
+      ((n_5) .& (temp_6)) in 
+     temp_9 ←
+      (nat_mod_from_secret_literal (n_5)) ;; 
+    let temp_8 := type_from_choice_type_elem temp_9 in
+    pkg_core_definition.ret (choice_type_from_type_elem (temp_8))
+    } : code ((fset [ n_5_loc])) [interface] _).
+Admit Obligations.
 
-Definition poly1305_encode_block (b_437 : poly_block_t) : field_element_t :=
-  let n_438 : uint128 :=
-    uint128_from_le_bytes (array_from_seq (16) (array_to_seq (b_437))) in 
-  let f_439 : field_element_t :=
-    nat_mod_from_secret_literal (n_438) in 
-  (f_439) +% (nat_mod_pow2 (0x03fffffffffffffffffffffffffffffffb) (
-      usize 128) : field_element_t).
 
-Definition poly1305_encode_last
-  (pad_len_440 : block_index_t)
-  (b_441 : sub_block_t)
-  : field_element_t :=
-  let n_442 : uint128 :=
-    uint128_from_le_bytes (array_from_slice (default) (16) (b_441) (usize 0) (
-        seq_len (b_441))) in 
-  let f_443 : field_element_t :=
-    nat_mod_from_secret_literal (n_442) in 
-  (f_443) +% (nat_mod_pow2 (0x03fffffffffffffffffffffffffffffffb) ((usize 8) * (
-        pad_len_440)) : field_element_t).
+Program Definition poly1305_encode_block
+  (b_13 : poly_block_t)
+  : code fset.fset0 [interface] (choice_type_from_type (field_element_t)) :=
+  ({code
+     temp_15 ←
+      (array_from_seq (16) (array_to_seq (b_13))) ;; 
+    let temp_14 := type_from_choice_type_elem temp_15 in
+     temp_17 ←
+      (uint128_from_le_bytes (temp_14)) ;; 
+    let temp_16 := type_from_choice_type_elem temp_17 in
+    let n_18 : uint128 :=
+      (temp_16) in 
+     temp_20 ←
+      (nat_mod_from_secret_literal (n_18)) ;; 
+    let temp_19 := type_from_choice_type_elem temp_20 in
+    let f_21 : field_element_t :=
+      (temp_19) in 
+     temp_23 ←
+      (nat_mod_pow2 (0x03fffffffffffffffffffffffffffffffb) (usize 128)) ;; 
+    let temp_22 := type_from_choice_type_elem temp_23 : field_element_t in
+    pkg_core_definition.ret (choice_type_from_type_elem ((f_21) +% (temp_22)))
+    } : code (fset.fset0) [interface] _).
+Admit Obligations.
 
-Definition poly1305_init (k_444 : poly_key_t) : poly_state_t :=
-  let r_445 : field_element_t :=
-    poly1305_encode_r (array_from_slice (default) (16) (array_to_seq (k_444)) (
-        usize 0) (usize 16)) in 
-  (nat_mod_zero , r_445, k_444).
 
-Definition poly1305_update_block
-  (b_446 : poly_block_t)
-  (st_447 : poly_state_t)
-  : poly_state_t :=
-  let '(acc_448, r_449, k_450) :=
-    st_447 in 
-  (((poly1305_encode_block (b_446)) +% (acc_448)) *% (r_449), r_449, k_450).
+Program Definition poly1305_encode_last
+  (pad_len_33 : block_index_t)
+  (b_24 : sub_block_t)
+  : code fset.fset0 [interface] (choice_type_from_type (field_element_t)) :=
+  ({code
+     temp_26 ←
+      (array_from_slice (default) (16) (b_24) (usize 0) (seq_len (b_24))) ;; 
+    let temp_25 := type_from_choice_type_elem temp_26 in
+     temp_28 ←
+      (uint128_from_le_bytes (temp_25)) ;; 
+    let temp_27 := type_from_choice_type_elem temp_28 in
+    let n_29 : uint128 :=
+      (temp_27) in 
+     temp_31 ←
+      (nat_mod_from_secret_literal (n_29)) ;; 
+    let temp_30 := type_from_choice_type_elem temp_31 in
+    let f_32 : field_element_t :=
+      (temp_30) in 
+     temp_35 ←
+      (nat_mod_pow2 (0x03fffffffffffffffffffffffffffffffb) ((usize 8) * (
+            pad_len_33))) ;; 
+    let temp_34 := type_from_choice_type_elem temp_35 : field_element_t in
+    pkg_core_definition.ret (choice_type_from_type_elem ((f_32) +% (temp_34)))
+    } : code (fset.fset0) [interface] _).
+Admit Obligations.
 
-Definition poly1305_update_blocks
-  (m_451 : byte_seq)
-  (st_452 : poly_state_t)
-  : poly_state_t :=
-  let st_453 : (field_element_t × field_element_t × poly_key_t) :=
-    st_452 in 
-  let n_blocks_454 : uint_size :=
-    (seq_len (m_451)) / (blocksize_v) in 
-  let st_453 :=
-    foldi (usize 0) (n_blocks_454) (fun i_455 st_453 =>
-      let block_456 : poly_block_t :=
-        array_from_seq (16) (seq_get_exact_chunk (m_451) (blocksize_v) (
-            i_455)) in 
-      let st_453 :=
-        poly1305_update_block (block_456) (st_453) in 
-      (st_453))
-    st_453 in 
-  st_453.
 
-Definition poly1305_update_last
-  (pad_len_457 : uint_size)
-  (b_458 : sub_block_t)
-  (st_459 : poly_state_t)
-  : poly_state_t :=
-  let st_460 : (field_element_t × field_element_t × poly_key_t) :=
-    st_459 in 
-  let '(st_460) :=
-    if (seq_len (b_458)) !=.? (usize 0):bool then (let '(acc_461, r_462, k_463
-        ) :=
-        st_460 in 
-      let st_460 :=
-        (
-          ((poly1305_encode_last (pad_len_457) (b_458)) +% (acc_461)) *% (
-            r_462),
-          r_462,
-          k_463
-        ) in 
-      (st_460)) else ((st_460)) in 
-  st_460.
+Program Definition poly1305_init
+  (k_36 : poly_key_t)
+  : code (fset [ n_5_loc]) [interface] (choice_type_from_type (poly_state_t)) :=
+  ({code
+     temp_38 ←
+      (array_from_slice (default) (16) (array_to_seq (k_36)) (usize 0) (
+          usize 16)) ;; 
+    let temp_37 := type_from_choice_type_elem temp_38 in
+     temp_40 ←
+      (poly1305_encode_r (temp_37)) ;; 
+    let temp_39 := type_from_choice_type_elem temp_40 in
+    let r_43 : field_element_t :=
+      (temp_39) in 
+     temp_42 ←
+      (nat_mod_zero ) ;; 
+    let temp_41 := type_from_choice_type_elem temp_42 in
+    pkg_core_definition.ret (choice_type_from_type_elem ((temp_41, r_43, k_36)))
+    } : code ((fset [ n_5_loc])) [interface] _).
+Admit Obligations.
 
-Definition poly1305_update
-  (m_464 : byte_seq)
-  (st_465 : poly_state_t)
-  : poly_state_t :=
-  let st_466 : (field_element_t × field_element_t × poly_key_t) :=
-    poly1305_update_blocks (m_464) (st_465) in 
-  let last_467 : seq uint8 :=
-    seq_get_remainder_chunk (m_464) (blocksize_v) in 
-  poly1305_update_last (seq_len (last_467)) (last_467) (st_466).
 
-Definition poly1305_finish (st_468 : poly_state_t) : poly1305_tag_t :=
-  let '(acc_469, _, k_470) :=
-    st_468 in 
-  let n_471 : uint128 :=
-    uint128_from_le_bytes (array_from_slice (default) (16) (
-        array_to_seq (k_470)) (usize 16) (usize 16)) in 
-  let aby_472 : seq uint8 :=
-    nat_mod_to_byte_seq_le (acc_469) in 
-  let a_473 : uint128 :=
-    uint128_from_le_bytes (array_from_slice (default) (16) (aby_472) (usize 0) (
-        usize 16)) in 
-  array_from_seq (16) (array_to_seq (uint128_to_le_bytes ((a_473) .+ (n_471)))).
+Program Definition poly1305_update_block
+  (b_47 : poly_block_t)
+  (st_46 : poly_state_t)
+  : code fset.fset0 [interface] (choice_type_from_type (poly_state_t)) :=
+  ({code
+    let '(acc_50, r_51, k_52) :=
+      (st_46) in 
+     temp_49 ←
+      (poly1305_encode_block (b_47)) ;; 
+    let temp_48 := type_from_choice_type_elem temp_49 in
+    pkg_core_definition.ret (choice_type_from_type_elem ((
+        ((temp_48) +% (acc_50)) *% (r_51),
+        r_51,
+        k_52
+      )))
+    } : code (fset.fset0) [interface] _).
+Admit Obligations.
 
-Definition poly1305
-  (m_474 : byte_seq)
-  (key_475 : poly_key_t)
-  : poly1305_tag_t :=
-  let st_476 : (field_element_t × field_element_t × poly_key_t) :=
-    poly1305_init (key_475) in 
-  let st_476 :=
-    poly1305_update (m_474) (st_476) in 
-  poly1305_finish (st_476).
+Definition st_60_loc : Location :=
+  (choice_type_from_type poly_state_t ; 66%nat).
+Program Definition poly1305_update_blocks
+  (m_54 : byte_seq)
+  (st_53 : poly_state_t)
+  : code (fset [ st_60_loc]) [interface] (choice_type_from_type (
+      poly_state_t)) :=
+  ({code
+    #put st_60_loc := choice_type_from_type_elem
+      (st_53) ;;
+    st_60 ← get st_60_loc ;;
+    let st_60 := type_from_choice_type_elem (st_60) in
+    let n_blocks_55 : uint_size :=
+      ((seq_len (m_54)) / (blocksize_v)) in 
+     temp_63 ←
+      (foldi (usize 0) (n_blocks_55) (fun i_56 st_60 =>
+          {code
+           temp_58 ←
+            (array_from_seq (16) (seq_get_exact_chunk (m_54) ( (blocksize_v)) (
+                   (i_56)))) ;; 
+          let temp_57 := type_from_choice_type_elem temp_58 in
+          let block_59 : poly_block_t :=
+            (temp_57) in 
+           temp_62 ←
+            (poly1305_update_block (block_59) (st_60)) ;; 
+          let temp_61 := type_from_choice_type_elem temp_62 in
+          let st_60 :=
+            (temp_61) in 
+          pkg_core_definition.ret (choice_type_from_type_elem ((st_60)))
+          } : code (fset.fset0) [interface] _)
+        st_60) ;; 
+    let st_60 := type_from_choice_type_elem temp_63 in
+    
+    pkg_core_definition.ret (choice_type_from_type_elem (st_60))
+    } : code ((fset [ st_60_loc])) [interface] _).
+Admit Obligations.
+
+Definition st_68_loc : Location :=
+  (choice_type_from_type poly_state_t ; 79%nat).
+Program Definition poly1305_update_last
+  (pad_len_70 : uint_size)
+  (b_69 : sub_block_t)
+  (st_67 : poly_state_t)
+  : code (fset [ st_68_loc]) [interface] (choice_type_from_type (
+      poly_state_t)) :=
+  ({code
+    #put st_68_loc := choice_type_from_type_elem
+      (st_67) ;;
+    st_68 ← get st_68_loc ;;
+    let st_68 := type_from_choice_type_elem (st_68) in
+     temp_76 ←
+      (if (seq_len (b_69)) !=.? (usize 0):bool then ({code
+          let '(acc_73, r_74, k_75) :=
+            (st_68) in 
+           temp_72 ←
+            (poly1305_encode_last (pad_len_70) (b_69)) ;; 
+          let temp_71 := type_from_choice_type_elem temp_72 in
+          let st_68 :=
+            ((((temp_71) +% (acc_73)) *% (r_74), r_74, k_75)) in 
+          pkg_core_definition.ret (choice_type_from_type_elem ((st_68)))
+          } : code (fset.fset0) [interface] _) else (
+          pkg_core_definition.ret (choice_type_from_type_elem ((st_68))))) ;; 
+    let '(st_68) := type_from_choice_type_elem temp_76 in
+    
+    pkg_core_definition.ret (choice_type_from_type_elem (st_68))
+    } : code ((fset [ st_68_loc])) [interface] _).
+Admit Obligations.
+
+
+Program Definition poly1305_update
+  (m_80 : byte_seq)
+  (st_81 : poly_state_t)
+  : code (fset [ st_60_loc ; st_68_loc]) [interface] (choice_type_from_type (
+      poly_state_t)) :=
+  ({code
+     temp_83 ←
+      (poly1305_update_blocks (m_80) (st_81)) ;; 
+    let temp_82 := type_from_choice_type_elem temp_83 in
+    let st_85 : (field_element_t '× field_element_t '× poly_key_t) :=
+      (temp_82) in 
+    let last_84 : seq uint8 :=
+      (seq_get_remainder_chunk (m_80) ( (blocksize_v))) in 
+     temp_87 ←
+      (poly1305_update_last (seq_len (last_84)) (last_84) (st_85)) ;; 
+    let temp_86 := type_from_choice_type_elem temp_87 in
+    pkg_core_definition.ret (choice_type_from_type_elem (temp_86))
+    } : code ((fset [ st_60_loc ; st_68_loc])) [interface] _).
+Admit Obligations.
+
+
+Program Definition poly1305_finish
+  (st_92 : poly_state_t)
+  : code fset.fset0 [interface] (choice_type_from_type (poly1305_tag_t)) :=
+  ({code
+    let '(acc_98, _, k_93) :=
+      (st_92) in 
+     temp_95 ←
+      (array_from_slice (default) (16) (array_to_seq (k_93)) (usize 16) (
+          usize 16)) ;; 
+    let temp_94 := type_from_choice_type_elem temp_95 in
+     temp_97 ←
+      (uint128_from_le_bytes (temp_94)) ;; 
+    let temp_96 := type_from_choice_type_elem temp_97 in
+    let n_105 : uint128 :=
+      (temp_96) in 
+    let aby_99 : seq uint8 :=
+      (nat_mod_to_byte_seq_le (acc_98)) in 
+     temp_101 ←
+      (array_from_slice (default) (16) (aby_99) (usize 0) (usize 16)) ;; 
+    let temp_100 := type_from_choice_type_elem temp_101 in
+     temp_103 ←
+      (uint128_from_le_bytes (temp_100)) ;; 
+    let temp_102 := type_from_choice_type_elem temp_103 in
+    let a_104 : uint128 :=
+      (temp_102) in 
+     temp_107 ←
+      (uint128_to_le_bytes ((a_104) .+ (n_105))) ;; 
+    let temp_106 := type_from_choice_type_elem temp_107 in
+     temp_109 ←
+      (array_from_seq (16) (array_to_seq (temp_106))) ;; 
+    let temp_108 := type_from_choice_type_elem temp_109 in
+    pkg_core_definition.ret (choice_type_from_type_elem (temp_108))
+    } : code (fset.fset0) [interface] _).
+Admit Obligations.
+
+Definition st_114_loc : Location :=
+  (choice_type_from_type poly_state_t ; 127%nat).
+Program Definition poly1305
+  (m_113 : byte_seq)
+  (key_110 : poly_key_t)
+  : code (fset [ n_5_loc ; st_114_loc ; st_60_loc ; st_68_loc]) [interface] (
+    choice_type_from_type (poly1305_tag_t)) :=
+  ({code
+     temp_112 ←
+      (poly1305_init (key_110)) ;; 
+    let temp_111 := type_from_choice_type_elem temp_112 in
+    #put st_114_loc := choice_type_from_type_elem
+      (temp_111) ;;
+    st_114 ← get st_114_loc ;;
+    let st_114 := type_from_choice_type_elem (st_114) in
+     temp_116 ←
+      (poly1305_update (m_113) (st_114)) ;; 
+    let temp_115 := type_from_choice_type_elem temp_116 in
+    let st_114 :=
+      (temp_115) in 
+     temp_118 ←
+      (poly1305_finish (st_114)) ;; 
+    let temp_117 := type_from_choice_type_elem temp_118 in
+    pkg_core_definition.ret (choice_type_from_type_elem (temp_117))
+    } : code ((
+        fset [ n_5_loc ; st_114_loc ; st_60_loc ; st_68_loc])) [interface] _).
+Admit Obligations.
 
